coq/CircuitCorrectness.v
@@ -40,11 +40,6 @@ Section CompilerCorrectness.
                    rwdata csigma)).
 
   Section OpCompile.
-    Lemma interp_circuit_cast {sz sz'}:
-      forall (h: sz = sz') (c: circuit sz),
-        interp_circuit (rew h in c) = rew h in (interp_circuit c).
-    Proof. destruct h; reflexivity. Defined.
-
     Ltac compile_op_t :=
       match goal with
       | _ => progress intros
@@ -58,13 +53,14 @@ Section CompilerCorrectness.
       | [  |- context[match ?d with _ => _ end] ] => is_var d; destruct d
       | [  |- context[match le_gt_dec ?x ?y with _ => _ end] ] => destruct (le_gt_dec x y)
       | [  |- context[eq_rect _ _ _ _ ?pr] ] => destruct pr
+      | _ => rewrite lco_proof
       | _ => solve [eauto]
       end.
 
     Theorem compile_unop_correct :
       forall fn c a,
         interp_circuit c = a ->
-        interp_circuit (compile_unop fn c) = CircuitPrimSpecs.sigma1 fn a.
+        interp_circuit (compile_unop lco.(lco_fn) fn c) = CircuitPrimSpecs.sigma1 fn a.
     Proof.
       destruct fn; repeat compile_op_t.
     Qed.
@@ -73,7 +69,7 @@ Section CompilerCorrectness.
       forall fn c1 c2 a1 a2,
         interp_circuit c1 = a1 ->
         interp_circuit c2 = a2 ->
-        interp_circuit (compile_binop fn c1 c2) = CircuitPrimSpecs.sigma2 fn a1 a2.
+        interp_circuit (compile_binop lco.(lco_fn) fn c1 c2) = CircuitPrimSpecs.sigma2 fn a1 a2.
     Proof.
       destruct fn; repeat compile_op_t.
     Qed.
